Most of Counter ported to disk semantics

systems/Counter.v
@@ -1,6 +1,8 @@
 Require Import Verdi.Verdi.
 Require Import Verdi.HandlerMonad.
 
+Require Import Cheerios.Cheerios.
+
 Local Arguments update {_} {_} _ _ _ _ _ : simpl never.
 
 Set Implicit Arguments.
@@ -29,38 +31,49 @@ Definition Data := nat.
 
 Definition init_Data := 0.
 
-Definition Handler (S : Type) := GenHandler (Name * Msg) S Output unit.
+Definition Handler (S A : Type) := GenHandler (Name * Msg) S Output A.
 
-Definition PrimaryNetHandler (m : Msg) : Handler Data :=
+Definition snapshot : Handler Data disk :=
+  s <- get ;; ret (serialize_top serialize s).
+
+(* Definition keep_disk : Handler Data := *)
+Definition PrimaryNetHandler (m : Msg) : Handler Data unit :=
   match m with
   | ack => write_output inc_executed
   | _ => nop
   end.
 
-Definition PrimaryInputHandler (i : Input) : Handler Data :=
+Definition PrimaryInputHandler (i : Input) : Handler Data unit :=
   match i with
   | request_inc => modify S ;; send (backup, inc)
   end.
 
-Definition BackupNetHandler (m : Msg) : Handler Data :=
+Definition BackupNetHandler (m : Msg) : Handler Data unit :=
   match m with
   | inc => modify S ;; send (primary, ack)
   | _ => nop
   end.
 
-Definition BackupInputHandler (i : Input) : Handler Data := nop.
+Definition BackupInputHandler (i : Input) : Handler Data unit := nop.
 
-Definition NetHandler (me : Name) (m : Msg) : Handler Data :=
+Definition NetHandler' (me : Name) (m : Msg) : Handler Data unit :=
   match me with
   | primary => PrimaryNetHandler m
   | backup => BackupNetHandler m
   end.
 
-Definition InputHandler (me : Name) (i : Input) : Handler Data :=
+Definition NetHandler (me : Name) (m : Msg) : Handler Data disk :=
+  NetHandler' me m ;;
+              snapshot.
+
+Definition InputHandler' (me : Name) (i : Input) : Handler Data unit :=
   match me with
   | primary => PrimaryInputHandler i
   | backup => BackupInputHandler i
   end.
+
+Definition InputHandler (me : Name) (i : Input) : Handler Data disk :=
+  InputHandler' me i;; snapshot.
 
 Instance Counter_BaseParams : BaseParams :=
   {
@@ -81,47 +94,50 @@ Proof.
   repeat constructor; simpl; intuition discriminate.
 Qed.
 
-Instance Counter_MultiParams : MultiParams Counter_BaseParams :=
+Instance Counter_MultiParams : DiskParams Counter_BaseParams :=
   {
-    name := Name;
-    name_eq_dec := Name_eq_dec;
-    msg := Msg;
-    msg_eq_dec := Msg_eq_dec;
-    nodes := Nodes;
-    all_names_nodes := all_Names_Nodes;
-    no_dup_nodes := NoDup_Nodes;
-    init_handlers := fun _ => init_Data;
-    net_handlers := fun dst src msg s =>
-                      runGenHandler_ignore s (NetHandler dst msg);
-    input_handlers := fun nm i s =>
-                      runGenHandler_ignore s (InputHandler nm i)
+    d_name := Name;
+    d_name_eq_dec := Name_eq_dec;
+    d_msg := Msg;
+    d_msg_eq_dec := Msg_eq_dec;
+    d_nodes := Nodes;
+    d_all_names_nodes := all_Names_Nodes;
+    d_no_dup_nodes := NoDup_Nodes;
+    d_init_handlers := fun _ => init_Data;
+    d_init_disk := fun _ => (serialize_top serialize 3);
+    d_net_handlers := fun dst src msg s =>
+                        match (runGenHandler s (NetHandler dst msg)) with
+                        | (dsk, out, d, l) => (out, d, l, dsk)
+                        end;
+    d_input_handlers := fun nm i s =>
+                          match runGenHandler s (InputHandler nm i) with
+                          | (dsk, out, d, l) => (out, d, l, dsk)
+                          end
   }.
-
-
 Lemma net_handlers_NetHandler :
-  forall h src m d os d' ms,
-    net_handlers h src m d = (os, d', ms) ->
-    NetHandler h m d = (tt, os, d', ms).
+  forall h src m d os d' ms dsk,
+    d_net_handlers h src m d = (os, d', ms, dsk) ->
+    NetHandler h m d = (dsk, os, d', ms).
 Proof.
   intros.
   simpl in *.
   monad_unfold.
   repeat break_let.
   find_inversion.
-  destruct u. auto.
+  auto.
 Qed.
 
 Lemma input_handlers_InputHandlers :
-  forall h i d os d' ms,
-    input_handlers h i d = (os, d', ms) ->
-    InputHandler h i d = (tt, os, d', ms).
+  forall h i d os d' ms dsk,
+    d_input_handlers h i d = (os, d', ms, dsk) ->
+    InputHandler h i d = (dsk, os, d', ms).
 Proof.
   intros.
   simpl in *.
   monad_unfold.
   repeat break_let.
   find_inversion.
-  destruct u. auto.
+  auto.
 Qed.
 
 Lemma PrimaryNetHandler_no_msgs :
@@ -134,10 +150,10 @@ Proof.
   break_match; find_inversion; auto.
 Qed.
 
-Definition inc_in_flight_to_backup (l : list packet) : nat :=
+Definition inc_in_flight_to_backup (l : list d_packet) : nat :=
   length (filterMap
-            (fun p => if msg_eq_dec (pBody p) inc
-                   then if name_eq_dec (pDst p) backup
+            (fun p => if d_msg_eq_dec (d_pBody p) inc
+                   then if d_name_eq_dec (d_pDst p) backup
                         then Some tt else None
                    else None)
             l).
@@ -155,7 +171,7 @@ Qed.
 
 Lemma inc_in_flight_to_backup_cons_primary_dst :
   forall p,
-    pDst p = primary ->
+    d_pDst p = primary ->
     inc_in_flight_to_backup [p] = 0.
 Proof.
   intros.
@@ -173,26 +189,26 @@ Qed.
 Lemma InputHandler_inc_in_flight_to_backup_preserved :
   forall h i d u o d' l,
     InputHandler h i d = (u, o, d', l) ->
-    d' = d + inc_in_flight_to_backup (send_packets h l).
+    d' = d + inc_in_flight_to_backup (d_send_packets h l).
 Proof.
-  unfold InputHandler, PrimaryInputHandler, BackupInputHandler.
+  unfold InputHandler, InputHandler', PrimaryInputHandler, BackupInputHandler, snapshot.
   simpl.
   intros.
   monad_unfold.
-  repeat break_match; find_inversion; compute; auto.
+  repeat break_match; repeat find_inversion; compute; auto.
   rewrite plus_comm. auto.
 Qed.
 
 Lemma NetHandler_inc_in_flight_to_backup_preserved :
   forall p d u o d' l,
-    NetHandler (pDst p) (pBody p) d = (u, o, d', l) ->
-    d' + inc_in_flight_to_backup (send_packets (pDst p) l) = d + inc_in_flight_to_backup [p].
+    NetHandler (d_pDst p) (d_pBody p) d = (u, o, d', l) ->
+    d' + inc_in_flight_to_backup (d_send_packets (d_pDst p) l) = d + inc_in_flight_to_backup [p].
 Proof.
-  unfold NetHandler, PrimaryNetHandler, BackupNetHandler.
+  unfold NetHandler, NetHandler', PrimaryNetHandler, BackupNetHandler.
   intros.
   monad_unfold.
   destruct p. simpl in *.
-  repeat break_match; find_inversion; simpl; try rewrite inc_in_flight_to_backup_nil;
+  repeat break_match; repeat find_inversion; simpl; try rewrite inc_in_flight_to_backup_nil;
   unfold Data in *; compute;
   auto with *.
 Qed.
@@ -202,9 +218,9 @@ Lemma InputHandler_backup_no_msgs :
     InputHandler backup i d = (u, o, d', l) ->
     l = [].
 Proof.
-  simpl. unfold BackupInputHandler.
+  simpl. unfold InputHandler, InputHandler', BackupInputHandler.
   intros.
-  monad_unfold.
+  unfold snapshot in *. monad_unfold.
   find_inversion.
   auto.
 Qed.
@@ -216,32 +232,40 @@ Proof.
   auto.
 Qed.
 
+
+
 Lemma backup_plus_network_eq_primary :
   forall net tr,
-    step_async_star (params := Counter_MultiParams) step_async_init net tr ->
-    nwState net backup + inc_in_flight_to_backup (nwPackets net) = nwState net primary.
+    step_async_disk_star (params := Counter_MultiParams)
+                         step_async_disk_init
+                         net tr -> 
+    nwdState net backup + inc_in_flight_to_backup (nwdPackets net) = nwdState net primary.
 Proof.
   intros.
-  remember step_async_init as y in *.
+  remember step_async_disk_init as y in *.
   revert Heqy.
   induction H using refl_trans_1n_trace_n1_ind; intros; subst.
   - reflexivity.
   - concludes.
     match goal with
-    | [ H : step_async _ _ _ |- _ ] => invc H
+    | [ H : step_async_disk _ _ _ |- _ ] => invc H
     end; simpl.
     + find_apply_lem_hyp net_handlers_NetHandler.
       find_copy_apply_lem_hyp NetHandler_inc_in_flight_to_backup_preserved.
       repeat find_rewrite.
       rewrite cons_is_app in IHrefl_trans_1n_trace1.
       repeat rewrite inc_in_flight_to_backup_app in *.
-      destruct (pDst p) eqn:?;
+      destruct (d_pDst p) eqn:?;
                try rewrite update_same;
         try rewrite update_diff by congruence;
-        unfold send_packets in *; simpl in *.
-      * erewrite PrimaryNetHandler_no_msgs with (ms := l) in * by eauto.
-        rewrite inc_in_flight_to_backup_cons_primary_dst in * by auto.
+        unfold d_send_packets in *; simpl in *.
+      * unfold NetHandler, snapshot, NetHandler' in *.
+        (* 
+        erewrite PrimaryNetHandler_no_msgs with (ms := l) in *1.
+
         simpl in *. rewrite inc_in_flight_to_backup_nil in *. auto with *.
+         *)
+        admit.
       * omega.
     + find_apply_lem_hyp input_handlers_InputHandlers.
       find_copy_apply_lem_hyp InputHandler_inc_in_flight_to_backup_preserved.
@@ -253,19 +277,19 @@ Proof.
       * omega.
       * erewrite InputHandler_backup_no_msgs with (l := l) by eauto.
         simpl. rewrite inc_in_flight_to_backup_nil. omega.
-Qed.
+Admitted.
 
 Theorem primary_ge_backup :
   forall net tr,
-    step_async_star (params := Counter_MultiParams) step_async_init net tr ->
-    nwState net backup <= nwState net primary.
+    step_async_disk_star (params := Counter_MultiParams) step_async_disk_init net tr ->
+    nwdState net backup <= nwdState net primary.
 Proof.
   intros.
   apply backup_plus_network_eq_primary in H.
   auto with *.
 Qed.
 
-Definition trace_inputs (tr : list (name * (input + list output))) : nat :=
+Definition trace_inputs (tr : list (d_name * (input + list output))) : nat :=
   length (filterMap (fun e => match e with
                            | (primary, inl i) => Some i
                            | _ => None
@@ -280,7 +304,7 @@ Proof.
   rewrite app_length. auto.
 Qed.
 
-Definition trace_outputs (tr : list (name * (input + list output))) : nat :=
+Definition trace_outputs (tr : list (d_name * (input + list output))) : nat :=
   length (filterMap (fun e => match e with
                            | (primary, inr [o]) => Some o
                            | _ => None
@@ -296,10 +320,10 @@ Proof.
   rewrite app_length. auto.
 Qed.
 
-Definition ack_in_flight_to_primary (l : list packet) : nat :=
+Definition ack_in_flight_to_primary (l : list d_packet) : nat :=
   length (filterMap
-            (fun p => if msg_eq_dec (pBody p) ack
-                   then if name_eq_dec (pDst p) primary
+            (fun p => if d_msg_eq_dec (d_pBody p) ack
+                   then if d_name_eq_dec (d_pDst p) primary
                         then Some tt else None
                    else None)
             l).
@@ -316,7 +340,7 @@ Qed.
 
 Lemma ack_in_flight_to_primary_backup :
   forall p,
-    pDst p = backup ->
+    d_pDst p = backup ->
     ack_in_flight_to_primary [p] = 0.
 Proof.
   intros.
@@ -331,30 +355,30 @@ Lemma InputHandler_trace_preserved :
     InputHandler h i d = (u, o, d', l) ->
     trace_inputs [(h, inl i)] =
     trace_outputs [(h, inr o)] +
-    inc_in_flight_to_backup (send_packets h l) +
-    ack_in_flight_to_primary (send_packets h l).
+    inc_in_flight_to_backup (d_send_packets h l) +
+    ack_in_flight_to_primary (d_send_packets h l).
 Proof.
-  unfold InputHandler, PrimaryInputHandler, BackupInputHandler.
+  unfold InputHandler, InputHandler', snapshot, PrimaryInputHandler, BackupInputHandler.
   simpl.
   intros.
   monad_unfold.
-  repeat break_match; find_inversion; compute; auto.
+  repeat break_match; repeat find_inversion; compute; auto.
 Qed.
 
 Lemma NetHandler_trace_preserved :
   forall p d u o d' l,
-    NetHandler (pDst p) (pBody p) d = (u, o, d', l) ->
+    NetHandler (d_pDst p) (d_pBody p) d = (u, o, d', l) ->
     inc_in_flight_to_backup [p] +
     ack_in_flight_to_primary [p] =
-    trace_outputs [((pDst p), inr o)] +
-    inc_in_flight_to_backup (send_packets (pDst p) l) +
-    ack_in_flight_to_primary (send_packets (pDst p) l).
+    trace_outputs [((d_pDst p), inr o)] +
+    inc_in_flight_to_backup (d_send_packets (d_pDst p) l) +
+    ack_in_flight_to_primary (d_send_packets (d_pDst p) l).
 Proof.
-  unfold NetHandler, PrimaryNetHandler, BackupNetHandler.
+  unfold NetHandler, NetHandler', snapshot, PrimaryNetHandler, BackupNetHandler.
   intros.
   monad_unfold.
   destruct p. simpl in *.
-  repeat break_match; find_inversion; simpl; try rewrite inc_in_flight_to_backup_nil;
+  repeat break_match; repeat find_inversion; simpl; try rewrite inc_in_flight_to_backup_nil;
   unfold Data in *; compute;
   auto with *.
 Qed.
@@ -386,19 +410,19 @@ Qed.
 
 Lemma inputs_eq_outputs_plus_inc_plus_ack :
   forall net tr,
-    step_async_star (params := Counter_MultiParams) step_async_init net tr ->
+    step_async_disk_star (params := Counter_MultiParams) step_async_disk_init net tr ->
     trace_inputs tr = trace_outputs tr +
-                      inc_in_flight_to_backup (nwPackets net) +
-                      ack_in_flight_to_primary (nwPackets net).
+                      inc_in_flight_to_backup (nwdPackets net) +
+                      ack_in_flight_to_primary (nwdPackets net).
 Proof.
   intros.
-  remember step_async_init as y in *.
+  remember step_async_disk_init as y in *.
   revert Heqy.
   induction H using refl_trans_1n_trace_n1_ind; intros; subst.
   - reflexivity.
   - concludes.
     match goal with
-    | [ H : step_async _ _ _ |- _ ] => invc H
+    | [ H : step_async_disk _ _ _ |- _ ] => invc H
     end; simpl.
     + find_apply_lem_hyp net_handlers_NetHandler.
       repeat find_rewrite.
@@ -408,7 +432,7 @@ Proof.
       repeat rewrite inc_in_flight_to_backup_app in *.
       repeat rewrite ack_in_flight_to_primary_app in *.
       find_apply_lem_hyp NetHandler_trace_preserved.
-      destruct (pDst p) eqn:?.
+      destruct (d_pDst p) eqn:?.
       * erewrite inc_in_flight_to_backup_cons_primary_dst in * by eauto.
         rewrite trace_inputs_output in *. simpl in  *. omega.
       * rewrite ack_in_flight_to_primary_backup in * by auto.
@@ -428,7 +452,7 @@ Qed.
 
 Theorem inputs_ge_outputs :
   forall net tr,
-    step_async_star (params := Counter_MultiParams) step_async_init net tr ->
+    step_async_disk_star (params := Counter_MultiParams) step_async_disk_init net tr ->
     trace_outputs tr <= trace_inputs tr.
 Proof.
   intros.
